Exercise 3.2 #1:
    1) The base case is n = 0
        Show that sumTo Zero = Zero
    2) The inductive case n+1
        Show that add sumTo n (n+1) = sumTo (n+1)

Exercise 3.2 #2:
    Yes, the definition of reverse is enough to prove that reverse(l1 @ l2) = reverse l2 @ reverse l1
    base case: reverse ([] @ l2) = reverse l2 @ reverse []
    
        reverse ([] @ l2) = reverse l2 @ reverse []
        reverse (l2) = reverse l2 @ reverse [] by property of @
        reverse (l2) = reverse l2 @ [] by def of reverse
        reverse l2 = reverse l2 by property of @

    inductive case: reverse (x::xs @ l2) = reverse l2 @ reverse x::xs

        reverse (x::xs @ l2) = reverse l2 @ reverse x::xs
        reverse ([x] @ xs @ l2) = reverse l2 @ reverse x::xs by properties of lists
        reverse (x :: (xs @ ls)) = = reverse l2 @ reverse x::xs by properties of lists
        reverse (xs @ l2) @ [x] = reverse l2 @ reverse x::xs by def of reverse
        reverse l2 @ reverse xs @ [x] = reverse l2 @ reverse x::xs by inductive hypothesis
        reverse l2 @ (reverse xs) :: [x] = reverse l2 @ reverse x::xs by associativity of @
        reverse l2 @ reverse x::xs = reverse l2 @ reverse x::xs by def of reverse

