Base case:
    Sigma(i=0, 0, i) =? (0 (0 + 1) / 2)
                   0 =? (0 (0 + 1) / 2) by definition of Sigma
                   0 == 0 by arithmatic
                QED

General case:
    Sigma(i=0, n, i) = (n (n + 1) / 2) -> Sigma(i=0, n+1, i) = ((n+1) ((n+1) + 1) / 2)

    Given: Sigma(i=0, n, i) = (n (n + 1) / 2)

    Sigma(i=0, n+1, i) = ((n+1) ((n+1) + 1) / 2)
    Sigma(i=0, n, i) + (n+1) = ((n+1) ((n+1) + 1) / 2) by definition of Sigma
    (n (n + 1) / 2) + (n+1) = ((n+1) ((n+1) + 1) / 2) by inductive hypothesis
    (n (n + 1) / 2) + 2(n+1) / 2 = ((n+1) ((n+1) + 1) / 2) by arithmatic
    (n (n + 1) + 2(n+1) / 2) = ((n+1) ((n+1) + 1) / 2) by arithmatic
    (n^2 + n + 2n + 2 / 2) = ((n+1) ((n+1) + 1) / 2) by arithmatic
    (n^2 + 3n + 2 / 2) = ((n+1) ((n+1) + 1) / 2) by arithmatic
    ((n+1)(n+2) / 2) = ((n+1) ((n+1) + 1) / 2) by arithmatic
    ((n+1)((n+1) + 1) / 2) = ((n+1) ((n+1) + 1) / 2) by arithmatic
    QED

P(n) : sumTo n = Sigma (i=0, n, i)

Base case:
    sumTo 0 = Sigma (i=0, 0, i)
          0 = Sigma (i=0, 0, i) by definition of sumTo
          0 = 0 by definition of Sigma

Inductive case:
    sumTo(n) = Sigma(i=0, n, i) -> sumTo (n+1) = Sigma (i=0, n+1, i)
    Given: sumTo n = Sigma (i=0, n, i)

    sumTo (n+1) = Sigma (i=0, n+1, i)
    (n+1) + sumTo((n+1) - 1) = Sigma (i=0, n+1, i) by definition of sigma
    (n+1) + sumTo(n) = Sigma (i=0, n+1, i) by arithmatic
    (n+1) + Sigma (i=0, n, i) = Sigma (i=0, n+1, i) by inductive hypothesis
    Sigma (i=0, n, i) + (n+1) = Sigma (i=0, n, i) + (n+1) by definition of sigma

P(Zero):
    toInt (add Zero n') = toInt Zero + toInt n'
    toInt n' = toInt Zero + toInt n' by definition of add
    toInt n' = 0 + toInt n' by definition of toInt
    toInt n' = toInt n' by arithmatic

Given: toInt (add n n') =toInt n + toInt n'

P(Succ n):
    toInt (add (Succ n) n') = toInt (Succ n) + toInt n'
    toInt (Succ (add n n')) = toInt (Succ n) + toInt n' by definition of add
    toInt (add n n') + 1 = toInt (Succ n) + toInt n' by definition of toInt
    toInt n + toInt n' + 1 = toInt (Succ n) + toInt n' by inductive hypothesis
    toInt n + 1 + toInt n' =  toInt (Succ n) + toInt n' by definition of Succ
    toInt n + 1 + toInt n' = toInt n + 1 + toInt n' by definition of Succ

