Exercise 1:
    Prove minTree t = minNEList (flatten t)
    Principle of Induction: for any t : 'a tree: P(t) holds if:
                            - P(Leaf v) holds, for any v
                            - P(l) and P(r) -> P(Fork (l, v, r)), for any v
    Base case to prove: minTree (Leaf v) = minNEList (flatten (Leaf v))
    
    Base case: 
        minTree (Leaf v) = minNEList (flatten (Leaf v))
        v = minNEList (flatten (Leaf v)) by def of minTree
        v = minNEList (One v) by def of flatten
        v = v by def of minNEList

    Inductive case to prove: Show minTree (Fork (l, v, r)) = minNEList (flatten Fork (l, v, r))
                                - given minTree (l) = minNEList (flatten l)
                                - given minTree (r) = minNEList (flatten r)

    Inductive case:
        minTree (Fork (l, v, r)) = minNEList (flatten Fork (l, v, r))
        min v min minTree l minTree r = minNEList (flatten Fork (l, v, r)) by def of minTree
        min v min minNEList (flatten l) minNEList (flatten r) = minNEList (flatten Fork (l, v, r)) by inductive hypothesis
        min minNEList flatten l min v flatten r = minNEList (flatten Fork (l, v, r)) by communativity of min
        min minNEList flatten l min v flatten r = minNEList (app (flatten l) app (One v flatten r)) by def of flatten
        min minNEList flatten l (minNEList (Cons (v, (flatten r)))) = minNEList (app (flatten l) app (One v flatten r)) by def of flatten
        minNEList (app flatten l Cons (v, (flatten r))) = minNEList (app (flatten l) app (One v flatten r)) by lemma proven below
        minNEList (app flatten l Cons (v, (flatten r))) = minNEList (app (flatten l) Cons(v, flatten r) by def of app


        Prove: min (minNEList l) (minNEList r) = minNEList (app l r)